src/HoareWeak.v
@@ -11,13 +11,21 @@ Set Implicit Arguments.
 
 (** ** Hoare logic *)
 
-Definition corr2_weak (T: Type) pr (pre: donecond T -> crashcond -> block_mem -> hashmap ->  @pred _ _ valuset) (p: prog T) :=
-  forall d bm hm tr donec crashc out,
-    pre donec crashc bm hm d
-  -> exec pr d bm hm p out tr
-  -> ((exists d' bm' hm' v, out = Finished d' bm' hm' v /\
-                  donec d' bm' hm' v) \/
-      (exists d' bm' hm', out = Crashed d' bm' hm' /\ crashc bm' hm' d'))/\
+Definition corr2_weak (T: Type) pr (pre: donecond T -> crashcond -> block_mem tagged_block -> hashmap ->  rawpred tagged_block) (p: prog T) :=
+  forall d dt dtb bm bt btb hm tr donec crashc out,
+    disk_merges_to dt d dtb
+  -> mem_merges_to bt bm btb
+  -> pre donec crashc btb hm dtb      
+  -> exec pr d dt bm bt p out tr
+  -> ((exists d' dt' dtb' bm' bt' btb'  v,
+         out = Finished d' dt' bm' bt' v /\
+         (disk_merges_to (AEQ:=addr_eq_dec)) dt' d' dtb' /\
+         (mem_merges_to (AEQ:=handle_eq_dec)) bt' bm' btb' /\                            
+         donec btb' v dtb') \/
+     (exists d' dt' dtb' bm' bt' btb', out = Crashed d' dt' bm' bt' /\
+         (disk_merges_to (AEQ:=addr_eq_dec)) dt' d' dtb' /\
+         (mem_merges_to (AEQ:=handle_eq_dec)) bt' bm' btb' /\
+         crashc btb' dtb'))/\
     trace_secure pr tr.
 
 Notation "'{{W' pr | pre 'W}}' p" := (corr2_weak pr pre p)
@@ -44,7 +52,7 @@ Notation "'{<W' e1 .. e2 , 'PERM' : pr 'PRE' : bm , hm , pre 'POST' : bm' , hm' 
            [[ done'_ = done_ ]] * [[ crash'_ = crash_ ]])
         (rx r_) ]] *
      [[ forall bm'' hm'' , (F_ * crash * [[ exists l, hashmap_subset l hm hm'' ]] *
-                       [[ bm c= bm'' ]] ) =p=> crash_ bm'' hm'' ]]
+                       [[ bm c= bm'' ]] ) =p=> crash_ bm'' ]]
      )) .. ))
    )%pred
    (Bind p1 rx)%pred)
@@ -66,7 +74,7 @@ Notation "'{<W' 'PERM' : pr 'PRE' : bm , hm , pre 'POST' : bm' , hm' , post 'CRA
            [[ bm c= bm' ]] * [[ done'_ = done_ ]] * [[ crash'_ = crash_ ]])
         (rx r_) ]] *
      [[ forall bm'' hm'' , (F_ * crash * [[ exists l, hashmap_subset l hm hm'' ]] *
-                      [[ bm c= bm'' ]]) =p=> crash_ bm'' hm'' ]]
+                      [[ bm c= bm'' ]]) =p=> crash_ bm'' ]]
    )%pred
    (Bind p1 rx)%pred)
     (at level 0, p1 at level 60, bm at level 0, bm' at level 0,
@@ -84,7 +92,7 @@ Notation "'{!<W' e1 .. e2 , 'PERM' : pr 'PRE' : bm , hm , pre 'POST' : bm' , hm'
            [[ bm c= bm' ]] * [[ done'_ = done_ ]] * [[ crash'_ = crash_ ]])
         (rx r_) ]] *
      [[ forall bm'' hm'' , (crash * [[ exists l, hashmap_subset l hm hm'' ]] *
-                      [[ bm c= bm'' ]]) =p=> crash_ bm'' hm'' ]]
+                      [[ bm c= bm'' ]]) =p=> crash_ bm'' ]]
      )) .. ))
    )%pred
    (Bind p1 rx)%pred)
@@ -104,7 +112,7 @@ Notation "'{!<W' 'PERM' : pr 'PRE' : bm , hm , pre 'POST' : bm' , hm' , post 'CR
            [[ bm c= bm' ]] * [[ done'_ = done_ ]] * [[ crash'_ = crash_ ]])
         (rx r_) ]] *
      [[ forall bm'' hm'' , (crash * [[ exists l, hashmap_subset l hm hm'' ]] *
-                      [[ bm c= bm'' ]]) =p=> crash_ bm'' hm'' ]]
+                      [[ bm c= bm'' ]]) =p=> crash_ bm'' ]]
    )%pred
    (Bind p1 rx)%pred)
     (at level 0, p1 at level 60, bm at level 0, bm' at level 0,
@@ -127,7 +135,7 @@ Notation "'{<W' e1 .. e2 , 'PERM' : pr 'PRE' : bm , hm , pre 'POST' : bm' , hm' 
      [[ forall realcrash bm'' hm'',
           crash_xform realcrash =p=> crash_xform crash ->
           (F_ * realcrash * [[ exists l, hashmap_subset l hm hm'' ]] *
-                       [[ bm c= bm'' ]] ) =p=> crash_ bm'' hm'' ]]
+                       [[ bm c= bm'' ]] ) =p=> crash_ bm'' ]]
      )) .. ))
    )%pred
    (Bind p1 rx)%pred)
@@ -137,29 +145,29 @@ Notation "'{<W' e1 .. e2 , 'PERM' : pr 'PRE' : bm , hm , pre 'POST' : bm' , hm' 
     e1 closed binder, e2 closed binder).
 
 Theorem corr2_to_corr2_weak:
-  forall T pr (pre: donecond T -> crashcond -> block_mem ->  hashmap -> @pred _ _ valuset) (p: prog T),
+  forall T pr (pre: donecond T -> crashcond -> block_mem tagged_block -> hashmap ->  rawpred tagged_block) (p: prog T),
   corr2 pr pre p ->
   corr2_weak pr pre p.
 Proof.
   unfold corr2, corr2_weak; intros.
-  specialize H with (1:=H0)(2:=H1); cleanup.
+  specialize H with (1:=H0)(2:=H1)(3:=H2)(4:=H3); cleanup.
   split; auto.
   apply only_public_operations_to_trace_secure; eauto.
 Qed.
   
 Theorem pimpl_ok2_weak:
-  forall T pr (pre pre':donecond T -> crashcond -> block_mem ->  hashmap -> @pred _ _ valuset) (p: prog T),
+  forall T pr (pre pre': donecond T -> crashcond -> block_mem tagged_block -> hashmap ->  rawpred tagged_block) (p: prog T),
   corr2_weak pr pre' p ->
   (forall done crash bm hm, pre done crash bm hm =p=>  pre' done crash bm hm) ->
   corr2_weak pr pre p.
 Proof.
   unfold corr2_weak; intros.
   eapply H; eauto.
-  apply H0; auto.
+  apply H0; eauto.
 Qed.
 
 Theorem pimpl_ok2_cont_weak:
-  forall T pr (pre pre': donecond T -> crashcond -> block_mem ->  hashmap ->  @pred _ _ valuset) A (k : A -> prog T) x y,
+  forall T pr (pre pre': donecond T -> crashcond -> block_mem tagged_block -> hashmap ->  rawpred tagged_block) A (k : A -> prog T) x y,
     corr2_weak pr pre' (k y) ->
     (forall done crash bm hm, pre done crash bm hm =p=>  pre' done crash bm hm) ->
     (forall done crash bm hm, pre done crash bm hm =p=> [x = y]) ->
@@ -168,22 +176,22 @@ Proof.
   unfold corr2_weak; intros.
   edestruct H1; eauto.
   eapply H; eauto.
-  apply H0; auto.
+  apply H0; eauto.
 Qed.
 
 Theorem pimpl_pre2_weak:
-  forall T pr pre' (pre: donecond T -> crashcond -> block_mem ->  hashmap ->  @pred _ _ valuset) (p: prog T),
+  forall T pr pre' (pre: donecond T -> crashcond -> block_mem tagged_block -> hashmap ->  rawpred tagged_block) (p: prog T),
     (forall done crash bm hm, pre done crash bm hm  =p=>  [corr2_weak pr (pre' done crash bm hm) p]) ->
     (forall done crash bm hm, pre done crash bm hm  =p=> pre' done crash bm hm done crash bm hm) ->
     corr2_weak pr pre p.
 Proof.
   unfold corr2_weak; intros.
   eapply H; eauto.
-  apply H0; auto.
+  apply H0; eauto.
 Qed.
 
 Theorem pre_false2_weak:
-  forall T pr (pre: donecond T -> crashcond -> block_mem ->  hashmap ->  @pred _ _ valuset) (p: prog T),
+  forall T pr (pre: donecond T -> crashcond -> block_mem tagged_block -> hashmap ->  rawpred tagged_block) (p: prog T),
     (forall done crash bm hm, pre done crash bm hm =p=>  [False]) ->
     corr2_weak pr pre p.
 Proof.
@@ -197,7 +205,7 @@ Theorem corr2_weak_exists:
     corr2_weak pr (fun done crash bm hm => exists a:T, pre done crash bm hm a)%pred p.
 Proof.
   unfold corr2_weak; intros.
-  destruct H0.
+  destruct H2.
   eapply H; eauto.
 Qed.
 
@@ -208,7 +216,7 @@ Theorem corr2_weak_forall:
 Proof.
   unfold corr2_weak; intros.
   eapply H; eauto.
-  exists a; auto.
+  exists a; eauto.
 Qed.
 
 Theorem corr2_weak_equivalence :
@@ -237,7 +245,7 @@ Proof.
   eapply pimpl_ok2_weak; [| apply H1].
   unfold corr2_weak in *.
   intros.
-  destruct H2; eauto.
+  destruct H4; eauto.
 Qed.
 
 Ltac monad_simpl_one_weak :=
